Make a distinct_reds without stack stuff

Launchbury/LaunchburyCombinedTagged.thy
@@ -119,9 +119,7 @@ obtain a more convenient induction rule.
 inductive distinct_reds :: "heap \<Rightarrow> Flag \<Rightarrow> Flag \<Rightarrow> var list \<Rightarrow> heap \<Rightarrow> bool" ("_/ \<Down>\<^sup>_\<^sup>_\<^sup>d\<^bsub>_\<^esub>/ _" [50,50,50,50,50] 50)
 where
   DLambda: "\<lbrakk>
-      distinctVars ((x, (Lam [y]. e)) # \<Gamma>);
-      distinct (x#S);
-      set S \<subseteq> heapVars \<Gamma>
+      distinctVars ((x, (Lam [y]. e)) # \<Gamma>)
   \<rbrakk> \<Longrightarrow> 
       (x, (Lam [y]. e)) # \<Gamma> \<Down>\<^sup>i\<^sup>u\<^sup>d\<^bsub>x#S\<^esub> (x, (Lam [y]. e)) # \<Gamma>" 
  | DApplication: "\<lbrakk>
@@ -132,10 +130,6 @@ where
       distinctVars ((n, Lam [z]. e') # (x, App (Var n) y) # \<Delta>);
       distinctVars ((x, e'[z ::= y]) # \<Delta>);
       distinctVars \<Theta>;
-      distinct (x#S);
-      distinct (n#x#S);
-      set S \<subseteq> heapVars \<Gamma>;
-      set S \<subseteq> heapVars \<Delta>;
       (n, e) # (x, App (Var n) y) # \<Gamma> \<Down>\<^sup>\<times>\<^sup>u\<^sup>d\<^bsub>n#x#S\<^esub> (n, Lam [z]. e') # (x, App (Var n) y) # \<Delta>;
       (x, e'[z ::= y]) # \<Delta> \<Down>\<^sup>\<times>\<^sup>u\<^sup>d\<^bsub>x#S\<^esub> \<Theta>
     \<rbrakk> \<Longrightarrow>
@@ -148,10 +142,6 @@ where
       distinctVars ((n, Lam [z]. e') # (x, App (Var n) y) # \<Delta>);
       distinctVars ((z,Var y) # (x, e') # \<Delta>);
       distinctVars \<Theta>;
-      distinct (x#S);
-      distinct (n#x#S);
-      set S \<subseteq> heapVars \<Gamma>;
-      set S \<subseteq> heapVars \<Delta>;
       (n, e) # (x, App (Var n) y) # \<Gamma> \<Down>\<^sup>\<surd>\<^sup>u\<^sup>d\<^bsub>n#x#S\<^esub> (n, Lam [z]. e') # (x, App (Var n) y) # \<Delta>;
       (z,Var y) # (x, e') # \<Delta> \<Down>\<^sup>\<surd>\<^sup>u\<^sup>d\<^bsub>x#S\<^esub> \<Theta>
     \<rbrakk> \<Longrightarrow>
@@ -161,10 +151,6 @@ where
       distinctVars ((x, Var y) # \<Gamma>);
       distinctVars ((y,z) # (x, Var y) # \<Delta>);
       distinctVars ((y,z) # (x, z) # \<Delta>);
-      distinct (x#S);
-      distinct (y#x#S);
-      set S \<subseteq> heapVars \<Gamma>;
-      set S \<subseteq> heapVars \<Delta>;
       (x, Var y) # \<Gamma> \<Down>\<^sup>i\<^sup>\<surd>\<^sup>d\<^bsub>y#x#S\<^esub> (y,z) # (x, Var y) # \<Delta>
    \<rbrakk> \<Longrightarrow>
       (x, Var y) # \<Gamma> \<Down>\<^sup>i\<^sup>\<surd>\<^sup>d\<^bsub>x#S\<^esub> (y,z) # (x,z) # \<Delta>"
@@ -175,10 +161,6 @@ where
       distinctVars ((n, e) # (x, Var y) # \<Gamma>);
       distinctVars ((n,z) # (x, Var y) # \<Delta>);
       distinctVars ((x, z) # \<Delta>);
-      distinct (x#S);
-      distinct (n#y#x#S);
-      set S \<subseteq> heapVars \<Gamma>;
-      set S \<subseteq> heapVars \<Delta>;
       (y,e) \<in> set \<Gamma>;
       (n, e) # (x, Var y) # \<Gamma> \<Down>\<^sup>i\<^sup>\<times>\<^sup>d\<^bsub>n#y#x#S\<^esub> (n,z) # (x, Var y) # \<Delta>
    \<rbrakk> \<Longrightarrow>
@@ -189,9 +171,6 @@ where
       distinctVars ((x, Let as body) # \<Gamma>);
       distinctVars ((x, body) # asToHeap as);
       distinctVars \<Delta>;
-      distinct (x#S);
-      set S \<subseteq> heapVars \<Gamma>;
-      set S \<subseteq> heapVars \<Delta>;
       (x, body) # asToHeap as @ \<Gamma> \<Down>\<^sup>i\<^sup>u\<^sup>d\<^bsub>x#S\<^esub> \<Delta>
    \<rbrakk> \<Longrightarrow>
       (x, Let as body) # \<Gamma> \<Down>\<^sup>i\<^sup>u\<^sup>d\<^bsub>x#S\<^esub> \<Delta>"
@@ -202,15 +181,9 @@ where
       distinctVars \<Gamma>';
       distinctVars \<Delta>;
       distinctVars \<Delta>';
-      distinct S;
-      set S \<subseteq> heapVars \<Gamma>;
-      set S \<subseteq> heapVars \<Delta>;
-      set S \<subseteq> heapVars \<Gamma>';
-      set S \<subseteq> heapVars \<Delta>';
       \<Gamma> \<Down>\<^sup>i\<^sup>u\<^sup>d\<^bsub>S\<^esub> \<Delta>
    \<rbrakk> \<Longrightarrow> 
       \<Gamma>' \<Down>\<^sup>i\<^sup>u\<^sup>d\<^bsub>S\<^esub> \<Delta>'"
-
 equivariance distinct_reds
 
 nominal_inductive distinct_reds
@@ -229,20 +202,8 @@ lemma distinct_redsD3:
   "\<Gamma> \<Down>\<^sup>i\<^sup>u\<^sup>d\<^bsub>S\<^esub> \<Delta> \<Longrightarrow> distinctVars \<Delta>"
   by (induct rule: distinct_reds.induct) simp_all
 
-lemma distinct_redsD4:
-  "\<Gamma> \<Down>\<^sup>i\<^sup>u\<^sup>d\<^bsub>S\<^esub> \<Delta> \<Longrightarrow> set S \<subseteq> heapVars \<Gamma>"
-  by (induct rule: distinct_reds.induct) auto
-
-lemma distinct_redsD5:
-  "\<Gamma> \<Down>\<^sup>i\<^sup>u\<^sup>d\<^bsub>S\<^esub> \<Delta> \<Longrightarrow> set S \<subseteq> heapVars \<Delta>"
-  by (induct rule: distinct_reds.induct) auto
-
-lemma distinct_redsD6:
-  "\<Gamma> \<Down>\<^sup>i\<^sup>u\<^sup>d\<^bsub>S\<^esub> \<Delta> \<Longrightarrow> distinct S"
-  by (induct rule: distinct_reds.induct) auto
-
 lemma distinct_redsI:
-  "\<Gamma> \<Down>\<^sup>i\<^sup>u\<^sup>\<surd>\<^bsub>S\<^esub> \<Delta> \<Longrightarrow> distinctVars \<Gamma> \<Longrightarrow> distinct S \<Longrightarrow> set S \<subseteq> heapVars \<Gamma> \<Longrightarrow> \<Gamma> \<Down>\<^sup>i\<^sup>u\<^sup>d\<^bsub>S\<^esub> \<Delta>"
+  "\<Gamma> \<Down>\<^sup>i\<^sup>u\<^sup>\<surd>\<^bsub>S\<^esub> \<Delta> \<Longrightarrow> distinctVars \<Gamma>  \<Longrightarrow> \<Gamma> \<Down>\<^sup>i\<^sup>u\<^sup>d\<^bsub>S\<^esub> \<Delta>"
 proof (nominal_induct \<Gamma> i u "\<surd>" S \<Delta> rule: reds.strong_induct)
 case Lambda thus ?case by (auto intro: DLambda)
 next
@@ -252,21 +213,17 @@ case (Application n \<Gamma> x e y S \<Delta> \<Theta> z u e')
   moreover
 
   from Application
-  have "distinctVars ((n, e) # (x, App (Var n) y) # \<Gamma>)" and
-       "distinct (n#x#S)" and 
-        "set (n # x # S) \<subseteq> heapVars ((n, e) # (x, App (Var n) y) # \<Gamma>)"
+  have "distinctVars ((n, e) # (x, App (Var n) y) # \<Gamma>)" 
     by (auto simp add: distinctVars_Cons heapVars_not_fresh set_not_fresh)
   note Application(17)[OF this]
   moreover
 
-  from distinct_redsD3[OF this]  distinct_redsD5[OF this] `atom n \<sharp> S`
-  have "distinctVars ((x, e'[z::=y]) # \<Delta>)" and "set (x # S) \<subseteq> heapVars ((x, e'[z::=y]) # \<Delta>)"
+  from distinct_redsD3[OF this]
+  have "distinctVars ((x, e'[z::=y]) # \<Delta>)"
     by (auto simp add: distinctVars_Cons heapVars_not_fresh set_not_fresh)
-  note Application(19)[OF this(1)  `distinct (x # S)` this(2)]
+  note Application(19)[OF this(1)]
   moreover
-  note `distinctVars ((x, App e y) # \<Gamma>)` `distinct (x#S)` `distinct (n#x#S)`
-  moreover
-  note `set (x # S) \<subseteq> heapVars ((x, e'[z::=y]) # \<Delta>)` `set (n # x # S) \<subseteq> heapVars ((n, e) # (x, App (Var n) y) # \<Gamma>)`
+  note `distinctVars ((x, App e y) # \<Gamma>)`
   ultimately
   show ?case
     by (auto intro: DApplication elim: distinct_redsD2 distinct_redsD3)
@@ -278,69 +235,60 @@ case (ApplicationInd n \<Gamma> x e y S \<Delta> \<Theta> z u e')
 
   from ApplicationInd
   have "distinctVars ((n, e) # (x, App (Var n) y) # \<Gamma>)"
-      and "distinct (n#x#S)"
-      and "set (n # x # S) \<subseteq> heapVars ((n, e) # (x, App (Var n) y) # \<Gamma>)"
     by (auto simp add: distinctVars_Cons heapVars_not_fresh set_not_fresh)
   note ApplicationInd(16)[OF this]
   moreover
 
-  from distinct_redsD3[OF this] `atom z \<sharp> x` `atom z \<sharp> \<Delta>` distinct_redsD5[OF this] `atom n \<sharp> S`
-  have "distinctVars ((z, Var y) # (x, e') # \<Delta>)" "set (x # S) \<subseteq> heapVars ((z, Var y) # (x, e') # \<Delta>)"
+  from distinct_redsD3[OF this] `atom z \<sharp> x` `atom z \<sharp> \<Delta>`
+  have "distinctVars ((z, Var y) # (x, e') # \<Delta>)"
     by (auto simp add: distinctVars_Cons heapVars_not_fresh set_not_fresh)
-  note ApplicationInd(18)[OF this(1) `distinct (x # S)` this(2)]
+  note ApplicationInd(18)[OF this(1)]
   moreover
-  note `distinctVars ((x, App e y) # \<Gamma>)` `distinct (x#S)` `distinct (n#x#S)`
-  moreover
-  note `set (n # x # S) \<subseteq> heapVars ((n, e) # (x, App (Var n) y) # \<Gamma>)`
-       `set (x # S) \<subseteq> heapVars ((z, Var y) # (x, e') # \<Delta>)`
+  note `distinctVars ((x, App e y) # \<Gamma>)`
   ultimately
   show ?case
-    apply (auto intro!: DApplicationInd elim:  distinct_redsD2 distinct_redsD3)
-    by (metis  `atom z \<sharp> S` set_mp set_not_fresh subset_insert)
+    by (auto intro!: DApplicationInd elim:  distinct_redsD2 distinct_redsD3)
 next
 case (Variable y x S \<Gamma> i z \<Delta>)
-  with stack_head_there[OF Variable(2)]
-  have "distinct (y # x # S)" and "set (y # x # S) \<subseteq> heapVars ((x, Var y) # \<Gamma>)" by auto
-  from Variable(3)[OF `distinctVars ((x, Var y) # \<Gamma>)` this ]
-        distinct_redsD5[OF Variable(3)[OF `distinctVars ((x, Var y) # \<Gamma>)` this ]]
+  from Variable(3)[OF `distinctVars ((x, Var y) # \<Gamma>)`]       
         `distinctVars ((x, Var y) # \<Gamma>)`
-        `distinct (x#S)` `y \<notin> set (x # S)` `set (x # S) \<subseteq> heapVars ((x, Var y) # \<Gamma>)`
+        `y \<notin> set (x # S)`
   show ?case
     by (auto intro!: DVariable dest: distinct_redsD3 simp add: distinctVars_Cons)
 next
 case (VariableNoUpd n \<Gamma> x y e S \<Delta> z i)
-  hence "distinctVars ((n,e) # (x, Var y) # \<Gamma>)" and "distinct (n # y # x # S)" and "set (n # y # x # S) \<subseteq> heapVars ((n, e) # (x, Var y) # \<Gamma>)"
+  hence "distinctVars ((n,e) # (x, Var y) # \<Gamma>)"
     by (auto simp add: set_not_fresh fresh_at_base heapVars_from_set heapVars_not_fresh simp add: distinctVars_Cons)
   with VariableNoUpd(1-7)
         VariableNoUpd(11)[OF this]
         `distinctVars ((x, Var y) # \<Gamma>)`
-        `distinct (x#S)` `y \<notin> set (x # S)` `(y,e) \<in> set \<Gamma>`
-        `set (n # y # x # S) \<subseteq> heapVars ((n, e) # (x, Var y) # \<Gamma>)` `set (x # S) \<subseteq> heapVars ((x, Var y) # \<Gamma>)`
+        `y \<notin> set (x # S)` `(y,e) \<in> set \<Gamma>`
   show ?case
-    by (auto intro!: DVariableNoUpd dest: distinct_redsD3 set_mp[OF distinct_redsD5]  simp add: heapVars_not_fresh set_not_fresh distinctVars_Cons fresh_Pair)
+    by (auto intro!: DVariableNoUpd dest: distinct_redsD3 simp add: heapVars_not_fresh set_not_fresh distinctVars_Cons fresh_Pair)
 next
 case (Let as \<Gamma> x body i u S \<Delta>)
   moreover
-  from Let(1-4,6,8)
-  have "distinctVars ((x, body) # asToHeap as @ \<Gamma>)" and "set (x # S) \<subseteq> heapVars ((x, body) # asToHeap as @ \<Gamma>)"
+  from Let(1-4,6)
+  have "distinctVars ((x, body) # asToHeap as @ \<Gamma>)"
     apply (auto simp add: distinctVars_Cons distinctVars_append dest: fresh_assn_distinct)
     by (metis (hide_lams, mono_tags) IntI all_not_in_conv fresh_assn_distinct fresh_star_Pair fresh_star_list(1) fresh_star_list(2)  heapVars_from_set in_set_conv_decomp let_binders_fresh)
   moreover
-  note Let(5)[OF this(1) `distinct (x # S)` this(2)]
+  note Let(5)[OF this(1)]
   ultimately
   show ?case
-    by (auto intro!: DLet dest: distinct_redsD3  set_mp[OF distinct_redsD5] simp add: distinctVars_Cons fresh_star_Pair)
+    by (auto intro!: DLet dest: distinct_redsD3 simp add: distinctVars_Cons fresh_star_Pair)
 next
 case (Permute \<Gamma> \<Gamma>' \<Delta> \<Delta>' i u S)
   thus ?case
     apply -
     apply (rule DPermute, assumption+)
-    apply (auto dest: distinct_redsD3 set_mp[OF distinct_redsD5] simp add: perm_distinctVars perm_heapVars)
+    apply (auto dest: distinct_redsD3  simp add: perm_distinctVars perm_heapVars)
     done
 qed
 
+
 lemma reds_pres_distinctVars:
-  "\<Gamma> \<Down>\<^sup>i\<^sup>u\<^sup>\<surd>\<^bsub>S\<^esub> \<Delta> \<Longrightarrow> distinctVars \<Gamma> \<Longrightarrow> distinct S \<Longrightarrow> set S \<subseteq> heapVars \<Gamma> \<Longrightarrow> distinctVars \<Delta>"
+  "\<Gamma> \<Down>\<^sup>i\<^sup>u\<^sup>\<surd>\<^bsub>S\<^esub> \<Delta> \<Longrightarrow> distinctVars \<Gamma> \<Longrightarrow> distinctVars \<Delta>"
 by (metis distinct_redsD3 distinct_redsI)
 
 lemmas reds_distinct_ind = distinct_reds.induct[OF distinct_redsI, consumes 2, case_names Lambda Application Variable Let]
@@ -358,10 +306,237 @@ text {* Heap entries are never removed. *}
 lemma reds_doesnt_forget:
  assumes "\<Gamma> \<Down>\<^sup>i\<^sup>u\<^sup>\<surd>\<^bsub>S\<^esub> \<Delta>"
  assumes "distinctVars \<Gamma>"
- assumes "distinct S"
- assumes "set S \<subseteq> heapVars \<Gamma>"
  shows "heapVars \<Gamma> \<subseteq> heapVars \<Delta>"
 by (rule reds_doesnt_forget'[OF distinct_redsI[OF assms]])+
+
+
+text {*
+This is the same semantics with even more requirements.
+*}
+
+
+inductive distinct2_reds :: "heap \<Rightarrow> Flag \<Rightarrow> Flag \<Rightarrow> var list \<Rightarrow> heap \<Rightarrow> bool" ("_/ \<Down>\<^sup>_\<^sup>_\<^sup>D\<^bsub>_\<^esub>/ _" [50,50,50,50,50] 50)
+where
+  DLambda: "\<lbrakk>
+      distinctVars ((x, (Lam [y]. e)) # \<Gamma>);
+      distinct (x#S);
+      set S \<subseteq> heapVars \<Gamma>
+  \<rbrakk> \<Longrightarrow> 
+      (x, (Lam [y]. e)) # \<Gamma> \<Down>\<^sup>i\<^sup>u\<^sup>D\<^bsub>x#S\<^esub> (x, (Lam [y]. e)) # \<Gamma>" 
+ | DApplication: "\<lbrakk>
+      atom n \<sharp> (\<Gamma>,x,e,y,S,\<Delta>,\<Theta>,z);
+      atom z \<sharp> (\<Gamma>,x,e,y,S,\<Delta>,\<Theta>);
+      distinctVars ((x, App e y) # \<Gamma>);
+      distinctVars ((n, e) # (x, App (Var n) y) # \<Gamma>);
+      distinctVars ((n, Lam [z]. e') # (x, App (Var n) y) # \<Delta>);
+      distinctVars ((x, e'[z ::= y]) # \<Delta>);
+      distinctVars \<Theta>;
+      distinct (x#S);
+      distinct (n#x#S);
+      set S \<subseteq> heapVars \<Gamma>;
+      set S \<subseteq> heapVars \<Delta>;
+      (n, e) # (x, App (Var n) y) # \<Gamma> \<Down>\<^sup>\<times>\<^sup>u\<^sup>D\<^bsub>n#x#S\<^esub> (n, Lam [z]. e') # (x, App (Var n) y) # \<Delta>;
+      (x, e'[z ::= y]) # \<Delta> \<Down>\<^sup>\<times>\<^sup>u\<^sup>D\<^bsub>x#S\<^esub> \<Theta>
+    \<rbrakk> \<Longrightarrow>
+      (x, App e y) # \<Gamma> \<Down>\<^sup>\<times>\<^sup>u\<^sup>D\<^bsub>x#S\<^esub> \<Theta>" 
+ | DApplicationInd: "\<lbrakk>
+      atom n \<sharp> (\<Gamma>,x,e,y,S,\<Delta>,\<Theta>,z);
+      atom z \<sharp> (\<Gamma>,x,e,y,S,\<Delta>);
+      distinctVars ((x, App e y) # \<Gamma>);
+      distinctVars ((n, e) # (x, App (Var n) y) # \<Gamma>);
+      distinctVars ((n, Lam [z]. e') # (x, App (Var n) y) # \<Delta>);
+      distinctVars ((z,Var y) # (x, e') # \<Delta>);
+      distinctVars \<Theta>;
+      distinct (x#S);
+      distinct (n#x#S);
+      set S \<subseteq> heapVars \<Gamma>;
+      set S \<subseteq> heapVars \<Delta>;
+      (n, e) # (x, App (Var n) y) # \<Gamma> \<Down>\<^sup>\<surd>\<^sup>u\<^sup>D\<^bsub>n#x#S\<^esub> (n, Lam [z]. e') # (x, App (Var n) y) # \<Delta>;
+      (z,Var y) # (x, e') # \<Delta> \<Down>\<^sup>\<surd>\<^sup>u\<^sup>D\<^bsub>x#S\<^esub> \<Theta>
+    \<rbrakk> \<Longrightarrow>
+      (x, App e y) # \<Gamma> \<Down>\<^sup>\<surd>\<^sup>u\<^sup>D\<^bsub>x#S\<^esub> \<Theta>" 
+ | DVariable: "\<lbrakk>
+      y \<notin> set (x#S);
+      distinctVars ((x, Var y) # \<Gamma>);
+      distinctVars ((y,z) # (x, Var y) # \<Delta>);
+      distinctVars ((y,z) # (x, z) # \<Delta>);
+      distinct (x#S);
+      distinct (y#x#S);
+      set S \<subseteq> heapVars \<Gamma>;
+      set S \<subseteq> heapVars \<Delta>;
+      (x, Var y) # \<Gamma> \<Down>\<^sup>i\<^sup>\<surd>\<^sup>D\<^bsub>y#x#S\<^esub> (y,z) # (x, Var y) # \<Delta>
+   \<rbrakk> \<Longrightarrow>
+      (x, Var y) # \<Gamma> \<Down>\<^sup>i\<^sup>\<surd>\<^sup>D\<^bsub>x#S\<^esub> (y,z) # (x,z) # \<Delta>"
+ | DVariableNoUpd: "\<lbrakk>
+      atom n \<sharp> (\<Gamma>,x,y,e,S,\<Delta>,z);
+      y \<notin> set (x#S);
+      distinctVars ((x, Var y) # \<Gamma>);
+      distinctVars ((n, e) # (x, Var y) # \<Gamma>);
+      distinctVars ((n,z) # (x, Var y) # \<Delta>);
+      distinctVars ((x, z) # \<Delta>);
+      distinct (x#S);
+      distinct (n#y#x#S);
+      set S \<subseteq> heapVars \<Gamma>;
+      set S \<subseteq> heapVars \<Delta>;
+      (y,e) \<in> set \<Gamma>;
+      (n, e) # (x, Var y) # \<Gamma> \<Down>\<^sup>i\<^sup>\<times>\<^sup>D\<^bsub>n#y#x#S\<^esub> (n,z) # (x, Var y) # \<Delta>
+   \<rbrakk> \<Longrightarrow>
+      (x, Var y) # \<Gamma> \<Down>\<^sup>i\<^sup>\<times>\<^sup>D\<^bsub>x#S\<^esub> (x,z) # \<Delta>"
+ | DLet: "\<lbrakk>
+      set (bn as) \<sharp>* (\<Gamma>, x);
+      distinctVars (asToHeap as);
+      distinctVars ((x, Let as body) # \<Gamma>);
+      distinctVars ((x, body) # asToHeap as);
+      distinctVars \<Delta>;
+      distinct (x#S);
+      set S \<subseteq> heapVars \<Gamma>;
+      set S \<subseteq> heapVars \<Delta>;
+      (x, body) # asToHeap as @ \<Gamma> \<Down>\<^sup>i\<^sup>u\<^sup>D\<^bsub>x#S\<^esub> \<Delta>
+   \<rbrakk> \<Longrightarrow>
+      (x, Let as body) # \<Gamma> \<Down>\<^sup>i\<^sup>u\<^sup>D\<^bsub>x#S\<^esub> \<Delta>"
+ | DPermute: "\<lbrakk>
+      \<Gamma> <~~> \<Gamma>';
+      \<Delta> <~~> \<Delta>';
+      distinctVars \<Gamma>;
+      distinctVars \<Gamma>';
+      distinctVars \<Delta>;
+      distinctVars \<Delta>';
+      distinct S;
+      set S \<subseteq> heapVars \<Gamma>;
+      set S \<subseteq> heapVars \<Delta>;
+      set S \<subseteq> heapVars \<Gamma>';
+      set S \<subseteq> heapVars \<Delta>';
+      \<Gamma> \<Down>\<^sup>i\<^sup>u\<^sup>D\<^bsub>S\<^esub> \<Delta>
+   \<rbrakk> \<Longrightarrow> 
+      \<Gamma>' \<Down>\<^sup>i\<^sup>u\<^sup>D\<^bsub>S\<^esub> \<Delta>'"
+
+equivariance distinct2_reds
+
+nominal_inductive distinct2_reds
+  avoids DApplication: "n" and "z" | DApplicationInd: "n" | DVariableNoUpd: "n"
+  by (auto simp add: fresh_star_def fresh_Cons fresh_Pair pure_fresh)
+
+lemma distinct2_redsD1:
+  "\<Gamma> \<Down>\<^sup>i\<^sup>u\<^sup>D\<^bsub>S\<^esub> \<Delta> \<Longrightarrow> \<Gamma> \<Down>\<^sup>i\<^sup>u\<^sup>\<surd>\<^bsub>S\<^esub> \<Delta>"
+  by (induct rule: distinct2_reds.induct) (blast intro: reds.intros)+
+
+lemma distinct2_redsD2:
+  "\<Gamma> \<Down>\<^sup>i\<^sup>u\<^sup>D\<^bsub>S\<^esub> \<Delta> \<Longrightarrow> distinctVars \<Gamma>"
+  by (induct rule: distinct2_reds.induct) simp_all
+
+lemma distinct2_redsD3:
+  "\<Gamma> \<Down>\<^sup>i\<^sup>u\<^sup>D\<^bsub>S\<^esub> \<Delta> \<Longrightarrow> distinctVars \<Delta>"
+  by (induct rule: distinct2_reds.induct) simp_all
+
+lemma distinct2_redsD4:
+  "\<Gamma> \<Down>\<^sup>i\<^sup>u\<^sup>D\<^bsub>S\<^esub> \<Delta> \<Longrightarrow> set S \<subseteq> heapVars \<Gamma>"
+  by (induct rule: distinct2_reds.induct) auto
+
+lemma distinct2_redsD5:
+  "\<Gamma> \<Down>\<^sup>i\<^sup>u\<^sup>D\<^bsub>S\<^esub> \<Delta> \<Longrightarrow> set S \<subseteq> heapVars \<Delta>"
+  by (induct rule: distinct2_reds.induct) auto
+
+lemma distinct2_redsD6:
+  "\<Gamma> \<Down>\<^sup>i\<^sup>u\<^sup>D\<^bsub>S\<^esub> \<Delta> \<Longrightarrow> distinct S"
+  by (induct rule: distinct2_reds.induct) auto
+
+lemma distinct2_redsI:
+  "\<Gamma> \<Down>\<^sup>i\<^sup>u\<^sup>\<surd>\<^bsub>S\<^esub> \<Delta> \<Longrightarrow> distinctVars \<Gamma> \<Longrightarrow> distinct S \<Longrightarrow> set S \<subseteq> heapVars \<Gamma> \<Longrightarrow> \<Gamma> \<Down>\<^sup>i\<^sup>u\<^sup>D\<^bsub>S\<^esub> \<Delta>"
+proof (nominal_induct \<Gamma> i u "\<surd>" S \<Delta> rule: reds.strong_induct)
+case Lambda thus ?case by (auto intro: DLambda)
+next
+case (Application n \<Gamma> x e y S \<Delta> \<Theta> z u e')
+  have "atom n \<sharp> (\<Gamma>, x, e, y, S, \<Delta>, \<Theta>, z)" and "atom z \<sharp> (\<Gamma>, x, e, y, S, \<Delta>, \<Theta>)"
+    using Application by simp+
+  moreover
+
+  from Application
+  have "distinctVars ((n, e) # (x, App (Var n) y) # \<Gamma>)" and
+       "distinct (n#x#S)" and 
+        "set (n # x # S) \<subseteq> heapVars ((n, e) # (x, App (Var n) y) # \<Gamma>)"
+    by (auto simp add: distinctVars_Cons heapVars_not_fresh set_not_fresh)
+  note Application(17)[OF this]
+  moreover
+
+  from distinct2_redsD3[OF this]  distinct2_redsD5[OF this] `atom n \<sharp> S`
+  have "distinctVars ((x, e'[z::=y]) # \<Delta>)" and "set (x # S) \<subseteq> heapVars ((x, e'[z::=y]) # \<Delta>)"
+    by (auto simp add: distinctVars_Cons heapVars_not_fresh set_not_fresh)
+  note Application(19)[OF this(1)  `distinct (x # S)` this(2)]
+  moreover
+  note `distinctVars ((x, App e y) # \<Gamma>)` `distinct (x#S)` `distinct (n#x#S)`
+  moreover
+  note `set (x # S) \<subseteq> heapVars ((x, e'[z::=y]) # \<Delta>)` `set (n # x # S) \<subseteq> heapVars ((n, e) # (x, App (Var n) y) # \<Gamma>)`
+  ultimately
+  show ?case
+    by (auto intro: DApplication elim: distinct2_redsD2 distinct2_redsD3)
+next
+case (ApplicationInd n \<Gamma> x e y S \<Delta> \<Theta> z u e')
+  have "atom n \<sharp> (\<Gamma>, x, e, y, S, \<Delta>, \<Theta>, z)" and "atom z \<sharp> (\<Gamma>, x, e, y, S, \<Delta>)"
+    using ApplicationInd by simp+
+  moreover
+
+  from ApplicationInd
+  have "distinctVars ((n, e) # (x, App (Var n) y) # \<Gamma>)"
+      and "distinct (n#x#S)"
+      and "set (n # x # S) \<subseteq> heapVars ((n, e) # (x, App (Var n) y) # \<Gamma>)"
+    by (auto simp add: distinctVars_Cons heapVars_not_fresh set_not_fresh)
+  note ApplicationInd(16)[OF this]
+  moreover
+
+  from distinct2_redsD3[OF this] `atom z \<sharp> x` `atom z \<sharp> \<Delta>` distinct2_redsD5[OF this] `atom n \<sharp> S`
+  have "distinctVars ((z, Var y) # (x, e') # \<Delta>)" "set (x # S) \<subseteq> heapVars ((z, Var y) # (x, e') # \<Delta>)"
+    by (auto simp add: distinctVars_Cons heapVars_not_fresh set_not_fresh)
+  note ApplicationInd(18)[OF this(1) `distinct (x # S)` this(2)]
+  moreover
+  note `distinctVars ((x, App e y) # \<Gamma>)` `distinct (x#S)` `distinct (n#x#S)`
+  moreover
+  note `set (n # x # S) \<subseteq> heapVars ((n, e) # (x, App (Var n) y) # \<Gamma>)`
+       `set (x # S) \<subseteq> heapVars ((z, Var y) # (x, e') # \<Delta>)`
+  ultimately
+  show ?case
+    apply (auto intro!: DApplicationInd elim:  distinct2_redsD2 distinct2_redsD3)
+    by (metis  `atom z \<sharp> S` set_mp set_not_fresh subset_insert)
+next
+case (Variable y x S \<Gamma> i z \<Delta>)
+  with stack_head_there[OF Variable(2)]
+  have "distinct (y # x # S)" and "set (y # x # S) \<subseteq> heapVars ((x, Var y) # \<Gamma>)" by auto
+  from Variable(3)[OF `distinctVars ((x, Var y) # \<Gamma>)` this ]
+        distinct2_redsD5[OF Variable(3)[OF `distinctVars ((x, Var y) # \<Gamma>)` this ]]
+        `distinctVars ((x, Var y) # \<Gamma>)`
+        `distinct (x#S)` `y \<notin> set (x # S)` `set (x # S) \<subseteq> heapVars ((x, Var y) # \<Gamma>)`
+  show ?case
+    by (auto intro!: DVariable dest: distinct2_redsD3 simp add: distinctVars_Cons)
+next
+case (VariableNoUpd n \<Gamma> x y e S \<Delta> z i)
+  hence "distinctVars ((n,e) # (x, Var y) # \<Gamma>)" and "distinct (n # y # x # S)" and "set (n # y # x # S) \<subseteq> heapVars ((n, e) # (x, Var y) # \<Gamma>)"
+    by (auto simp add: set_not_fresh fresh_at_base heapVars_from_set heapVars_not_fresh simp add: distinctVars_Cons)
+  with VariableNoUpd(1-7)
+        VariableNoUpd(11)[OF this]
+        `distinctVars ((x, Var y) # \<Gamma>)`
+        `distinct (x#S)` `y \<notin> set (x # S)` `(y,e) \<in> set \<Gamma>`
+        `set (n # y # x # S) \<subseteq> heapVars ((n, e) # (x, Var y) # \<Gamma>)` `set (x # S) \<subseteq> heapVars ((x, Var y) # \<Gamma>)`
+  show ?case
+    by (auto intro!: DVariableNoUpd dest: distinct2_redsD3 set_mp[OF distinct2_redsD5]  simp add: heapVars_not_fresh set_not_fresh distinctVars_Cons fresh_Pair)
+next
+case (Let as \<Gamma> x body i u S \<Delta>)
+  moreover
+  from Let(1-4,6,8)
+  have "distinctVars ((x, body) # asToHeap as @ \<Gamma>)" and "set (x # S) \<subseteq> heapVars ((x, body) # asToHeap as @ \<Gamma>)"
+    apply (auto simp add: distinctVars_Cons distinctVars_append dest: fresh_assn_distinct)
+    by (metis (hide_lams, mono_tags) IntI all_not_in_conv fresh_assn_distinct fresh_star_Pair fresh_star_list(1) fresh_star_list(2)  heapVars_from_set in_set_conv_decomp let_binders_fresh)
+  moreover
+  note Let(5)[OF this(1) `distinct (x # S)` this(2)]
+  ultimately
+  show ?case
+    by (auto intro!: DLet dest: distinct2_redsD3  set_mp[OF distinct2_redsD5] simp add: distinctVars_Cons fresh_star_Pair)
+next
+case (Permute \<Gamma> \<Gamma>' \<Delta> \<Delta>' i u S)
+  thus ?case
+    apply -
+    apply (rule DPermute, assumption+)
+    apply (auto dest: distinct2_redsD3 set_mp[OF distinct2_redsD5] simp add: perm_distinctVars perm_heapVars)
+    done
+qed
 
 text {* The stack is never empty. *}
 
@@ -402,20 +577,20 @@ case (DApplication n \<Gamma> x e y S \<Delta> \<Theta> z e' u x')
   from `atom n \<sharp> x'` `atom x' \<sharp> (x, App e y) # \<Gamma>`
   have "atom x' \<sharp> (n, e) # (x, App (Var n) y) # \<Gamma>"
     by (auto simp add: fresh_Pair fresh_Cons)
-  from DApplication.hyps(28)[OF this]
+  from DApplication.hyps(24)[OF this]
   show ?case
   proof
     assume "atom x' \<sharp> (n, Lam [z]. e') # (x, App (Var n) y) # \<Delta>"
     with `atom z \<sharp> x'`
     have "atom x' \<sharp> (x, e'[z::=y]) # \<Delta>"
       by (simp add: fresh_Cons fresh_Pair subst_pres_fresh fresh_at_base)
-    from DApplication.hyps(30)[OF this]
+    from DApplication.hyps(26)[OF this]
     show ?thesis.
   next
     assume "x' \<in> heapVars ((n, Lam [z]. e') # (x, App (Var n) y) # \<Delta>)"
     with `atom n \<sharp> x'`
     have "x' \<in> heapVars ((x, e'[z::=y]) # \<Delta>)" by (simp add: fresh_at_base)
-    with reds_doesnt_forget'[OF DApplication(29)]
+    with reds_doesnt_forget'[OF DApplication(25)]
     have "x' \<in> heapVars \<Theta>" by auto
     thus ?thesis..
   qed
@@ -424,27 +599,27 @@ case (DApplicationInd n \<Gamma> x e y S \<Delta> \<Theta> z e' u x')
   show ?case
   proof(cases "x' = z")
   case True
-    with  reds_doesnt_forget'[OF DApplicationInd(27)]
+    with  reds_doesnt_forget'[OF DApplicationInd(23)]
     have "x' \<in> heapVars \<Theta>" by auto
     thus ?thesis..
   next
   case False
     hence "atom x' \<sharp> (n, e) # (x, App (Var n) y) # \<Gamma>"
       using DApplicationInd by (auto simp add: fresh_Pair fresh_Cons)
-    from DApplicationInd.hyps(26)[OF this]
+    from DApplicationInd.hyps(22)[OF this]
     show ?thesis
     proof
       assume "atom x' \<sharp> (n, Lam [z]. e') # (x, App (Var n) y) # \<Delta>"
       with `atom n \<sharp> x'` `x' \<noteq> z`
       have "atom x' \<sharp> (z, Var y) # (x, e') # \<Delta>"
         by (simp add: fresh_Cons fresh_Pair subst_pres_fresh fresh_at_base)
-      from DApplicationInd.hyps(28)[OF this]
+      from DApplicationInd.hyps(24)[OF this]
       show ?thesis.
     next
       assume "x' \<in> heapVars ((n, Lam [z]. e') # (x, App (Var n) y) # \<Delta>)"
       with `atom n \<sharp> x'`
       have "x' \<in> heapVars ((z,Var y) # (x, e') # \<Delta>)" by (simp add: fresh_at_base)
-      with reds_doesnt_forget'[OF DApplicationInd(27)]
+      with reds_doesnt_forget'[OF DApplicationInd(23)]
       have "x' \<in> heapVars \<Theta>" by auto
       thus ?thesis..
     qed
@@ -460,7 +635,7 @@ case (DLet as \<Gamma> x body \<Delta> S i u x')
   show ?case
   proof(cases "x' \<in> heapVars (asToHeap as)")
     case True
-    with reds_doesnt_forget'[OF DLet(10)]
+    with reds_doesnt_forget'[OF DLet(7)]
     show ?thesis by auto
   next
     case False
@@ -468,7 +643,7 @@ case (DLet as \<Gamma> x body \<Delta> S i u x')
     with `atom x' \<sharp> (x, Let as body) # \<Gamma>`
     have "atom x' \<sharp> (x, body) # asToHeap as @ \<Gamma>"
       by (auto simp add: fresh_Cons fresh_Pair fresh_append fresh_fun_eqvt_app asToHeap_eqvt)
-    from DLet(11)[OF this]
+    from DLet(8)[OF this]
     show ?thesis.
   qed
 next 
